FokkerChallenge/EnhancedCslib/Basic.lean
@@ -1,0 +1,55 @@
+import Cslib.Languages.LambdaCalculus.LocallyNameless.Untyped.Basic
+import Cslib.Languages.LambdaCalculus.LocallyNameless.Untyped.FullBeta
+import Cslib.Languages.LambdaCalculus.LocallyNameless.Untyped.Congruence
+import Mathlib.Data.Finset.Lattice.Basic
+
+namespace Cslib
+
+namespace LambdaCalculus.LocallyNameless.Untyped.Term
+
+theorem openRec_fv_cases {M N: Term String} :
+(i: Nat) ->
+(openRec i N M).fv = M.fv \/
+(openRec i N M).fv = M.fv ∪ N.fv := by
+induction M with unfold openRec
+| bvar _ => intros i
+            split
+            simp
+            tauto
+| fvar _ => tauto
+| abs _ ih => intros i
+              conv =>
+                lhs
+                unfold fv
+              conv =>
+                rhs
+                lhs
+                unfold fv
+              conv =>
+                rhs
+                rhs
+                lhs
+                unfold fv
+              apply ih
+| app a b iha ihb =>  intros i
+                      conv =>
+                        lhs
+                        unfold fv
+                      conv =>
+                        rhs
+                        lhs
+                        unfold fv
+                      conv =>
+                        rhs
+                        rhs
+                        lhs
+                        unfold fv
+                      specialize iha i
+                      specialize ihb i
+                      cases iha <;> cases ihb <;> grind
+
+end Term
+
+end LambdaCalculus.LocallyNameless.Untyped
+
+end Cslib
