FokkerChallenge/EnhancedCslib/DoubleEta.lean
@@ -9,6 +9,7 @@ namespace Cslib
 
 namespace LambdaCalculus.LocallyNameless.Untyped.Term
 
+/-
 -- Not sure we really need this
 -- Not sure this theorem is correct: we might need eta-equal rather than eta-reduction
 -- eta-equal is not defined in cslib
@@ -20,7 +21,10 @@ y ∉ M.fv ∪ N.fv ->
 x ≠ y ->
 Relation.ReflTransGen FullBetaEta (Term.app (Term.app M (Term.fvar x)) (Term.fvar y)) (openRec 1 (Term.fvar y) (openRec 0 (Term.fvar x) N))) ->
 Relation.ReflTransGen FullBetaEta M N.abs.abs := by
+-- 应该不需要证明
+-- 在 apply Xi.abs 的时候, 会自然出现这个目标
 sorry
+-/
 
 end LambdaCalculus.LocallyNameless.Untyped.Term
 
